coq/Imp/Lang/ImpJsonEval.v
@@ -25,6 +25,7 @@ Require Import Arith.
 Require Import EquivDec.
 Require Import Morphisms.
 Require Import Arith.
+Require Import ZArith.
 Require Import Max.
 Require Import Bool.
 Require Import Peano_dec.
@@ -33,22 +34,196 @@ Require Import Decidable.
 Require Import Utils.
 Require Import CommonRuntime.
 Require Import Imp.
+Require Import ImpEval.
 Require Import ImpJson.
 
 Section ImpJsonEval.
 
-  Context {fruntime:foreign_runtime}.
-
-  (* Context (h:brand_relation_t). *)
-
-  (* Local Open Scope imp_json. *)
   Local Open Scope string.
+
+  Section EvalInstantiation.
+    (* Instantiate Imp for Qcert data *)
+    Definition imp_json_data_normalize (d:imp_json_data) : imp_json_data :=
+      d. (* XXX What to do? *)
+
+    Definition imp_json_data_to_bool (d:imp_json_data) : option bool :=
+      match d with
+      | jbool b => Some b
+      | _ => None
+      end.
+
+    Definition imp_json_data_to_Z (d:imp_json_data) : option Z :=
+      match d with
+      | jnumber n => Some (float_truncate n)
+      | _ => None
+      end.
+
+    Definition of_string_list (sl:list json) : option (list string)
+      := lift_map (fun x => match x with jstring s => Some s | _ => None end) sl.
+    
+    Definition imp_json_runtime_eval (rt:imp_json_runtime_op) (dl:list imp_json_data) : option imp_json_data :=
+      match rt with
+      | JSONRuntimeEqual =>
+        apply_binary (fun d1 d2 => if json_eq_dec d1 d2 then Some (jbool true) else Some (jbool false)) dl
+      | JSONRuntimeCompare => None (* XXX pfff... *)
+      | JSONRuntimeRecConcat =>
+        apply_binary
+          (fun d1 d2 =>
+             match d1, d2 with
+             | (jobject r1), (jobject r2) => Some (jobject (rec_sort (r1++r2)))
+             | _, _ => None
+             end) dl
+      | JSONRuntimeRecMerge =>
+        apply_binary
+          (fun d1 d2 =>
+             match d1, d2 with
+             | (jobject r1), (jobject r2) =>
+               match @merge_bindings json _ json_eq_dec r1 r2 with
+               | Some x => Some (jarray ((jobject x) :: nil))
+               | None => Some (jarray nil)
+               end
+             | _, _ => None
+             end) dl
+      | JSONRuntimeDistinct =>
+        apply_unary
+          (fun d =>
+             match d with
+             | jarray l =>
+               Some (jarray (@bdistinct json json_eq_dec l))
+             | _ => None
+             end)
+          dl
+      | JSONRuntimeGroupBy => None (* XXX TODO *)
+      | JSONRuntimeDeref => (* XXX the one in qcert-runtime is a lot more complex *)
+        apply_binary
+          (fun d1 d2 =>
+             match d1, d2 with
+             | jobject r, jstring s =>
+               edot r s
+             | _, _ => None
+             end) dl
+      | JSONRuntimeEither =>
+        apply_unary
+          (fun d =>
+             match d with
+             | jobject (("left", _)::nil) => Some (jbool true)
+             | jobject (("right",_)::nil) => Some (jbool false)
+             | _ => None
+             end) dl
+      | JSONRuntimeToLeft =>
+        apply_unary
+          (fun d =>
+             match d with
+             | jobject (("left", d)::nil) => Some d
+             | _ => None
+             end) dl
+      | JSONRuntimeToRight =>
+        apply_unary
+          (fun d =>
+             match d with
+             | jobject (("right", d)::nil) => Some d
+             | _ => None
+             end) dl
+      | JSONRuntimeRemove =>
+        apply_binary
+          (fun d1 d2 =>
+             match d1, d2 with
+             | jobject r, jstring s =>
+               Some (jobject (rremove r s))
+             | _, _ => None
+             end) dl
+      | JSONRuntimeProject =>
+        apply_binary
+          (fun d1 d2 =>
+             match d1, d2 with
+             | jobject r, jarray sl =>
+               lift jobject (lift (rproject r) (of_string_list sl))
+             | _, _ => None
+             end) dl
+      | JSONRuntimeSingleton =>
+        apply_unary
+          (fun d =>
+             match d with
+             | jarray (d::nil) => Some d
+             | _ => None
+             end) dl
+      | JSONRuntimeFlatten => None
+      | JSONRuntimeSort => None
+      | JSONRuntimeCount => None
+      | JSONRuntimeLength => None
+      | JSONRuntimeSubstring => None
+      | JSONRuntimeBrand => None
+      | JSONRuntimeUnbrand => None
+      | JSONRuntimeCast => None
+      | JSONRuntimeNatPlus => None
+      | JSONRuntimeNatMinus => None
+      | JSONRuntimeNatMult => None
+      | JSONRuntimeNatDiv => None
+      | JSONRuntimeNatRem => None
+      | JSONRuntimeNatAbs => None
+      | JSONRuntimeNatLog2 => None
+      | JSONRuntimeNatSqrt => None
+      | JSONRuntimeNatSum => None
+      | JSONRuntimeNatMin => None
+      | JSONRuntimeNatMax => None
+      | JSONRuntimeNatArithMean => None
+      | JSONRuntimeFloatOfNat => None
+      | JSONRuntimeSum => None
+      | JSONRuntimeArithMean => None
+      | JSONRuntimeBunion => None
+      | JSONRuntimeBminus => None
+      | JSONRuntimeBmin => None
+      | JSONRuntimeBmax => None
+      | JSONRuntimeBnth => None
+      | JSONRuntimeContains => None
+      | JSONRuntimeToString => None
+      | JSONRuntimeGenerateText => None
+      end.
+
+    Definition imp_json_op_eval (op:imp_json_op) (dl:list imp_json_data) : option imp_json_data :=
+      json_op_eval op dl. (* XXX In Utils.JSONOperators *)
+
+  End EvalInstantiation.
 
   (** ** Evaluation Semantics *)
   Section Evaluation.
 
-    Definition imp_json_eval_top (* (σc:bindings) *) (q:imp_json) : option data (* XXX should be: json!!! XXX *) :=
-       None. (* XXX TODO XXX *)
+    (** Evaluation takes a ImpQcert expression and an environment. It
+          returns an optional value. When [None] is returned, it
+          denotes an error. An error is always propagated. *)
+
+    Definition jbindings := list (string * imp_json_data).
+    Definition pd_jbindings := list (string * option imp_json_data).
+    
+    Definition imp_json_expr_eval
+             (σc:jbindings) (σ:pd_jbindings) (e:imp_json_expr)
+    : option imp_json_data
+      := @imp_expr_eval
+           imp_json_data
+           imp_json_op
+           imp_json_runtime_op
+           imp_json_data_normalize
+           imp_json_runtime_eval
+           imp_json_op_eval
+           σc σ e.
+
+    Definition imp_json_stmt_eval
+             (σc:jbindings) (s:imp_json_stmt) (σ:pd_jbindings) : option (pd_jbindings)
+      := @imp_stmt_eval
+           imp_json_data
+           imp_json_op
+           imp_json_runtime_op
+           imp_json_data_normalize
+           imp_json_data_to_bool
+           imp_json_runtime_eval
+           imp_json_op_eval
+           σc s σ.
+
+    Definition imp_json_eval (σc:jbindings) (q:imp_json) : option (option imp_json_data)
+      := None. (* XXX TODO XXX *)
+
+    Definition imp_json_eval_top σc (q:imp_json) :=
+      olift id (imp_json_eval (rec_sort σc) q).
 
   End Evaluation.
 
